internal/LobsTheoremPreProof.v
@@ -1,0 +1,408 @@
+Require Import Coq.Setoids.Setoid Coq.Classes.Morphisms.
+Require Export Lob.Notations Lob.LobsTheoremStatement.
+
+(** The proof of the theorem *)
+
+Module Type LobExtendedContext <: LobContext.
+  Axiom Preterm : Type.
+  Axiom Context : Type.
+
+  Delimit Scope context_scope with ctx.
+  Bind Scope context_scope with Context.
+
+  Axiom empty_context : Context.
+  Notation ε := empty_context.
+  Axiom context_extend : Context -> Preterm -> Context.
+  Notation "Γ ▻ x" := (context_extend Γ x).
+
+  Delimit Scope preterm_scope with preterm.
+  Bind Scope preterm_scope with Preterm.
+
+  Global Open Scope preterm_scope.
+
+  Axiom box' : Context -> Preterm -> Type.
+
+  Definition box : Preterm -> Type
+    := box' ε.
+
+  Delimit Scope well_typed_term_scope with wtt.
+  Bind Scope well_typed_term_scope with box'.
+  Bind Scope well_typed_term_scope with box.
+
+  Notation "□ T" := (box T).
+
+
+  Axiom qbox : Preterm.
+  Notation "‘□’" := qbox.
+
+  Axiom tProd : Preterm -> Preterm -> Preterm.
+  Notation "x ‘→’ y" := (tProd x y) : preterm_scope.
+
+  Axiom tApp : Preterm -> Preterm -> Preterm.
+  Notation "x ‘’ y" := (tApp x y) : preterm_scope.
+
+  Axiom quote : Preterm -> Preterm.
+  Notation "⌜ x ⌝" := (quote x).
+
+
+  Delimit Scope well_typed_term_scope with wtt.
+  Bind Scope well_typed_term_scope with box'.
+End LobExtendedContext.
+
+Module Type PretermPrimitives (Export LC : LobExtendedContext).
+  Axiom tLambda : Preterm -> Preterm -> Preterm.
+  Axiom qtApp : Preterm.
+
+  Notation "‘App’" := qtApp : preterm_scope.
+
+  Axiom qtProd : Preterm -> Preterm -> Preterm.
+  Notation "x ‘‘→’’ y" := (qtProd x y) : preterm_scope.
+
+  Axiom ttVar0 : forall {Γ T}, box' (Γ ▻ T) T.
+  Notation "‘‘VAR₀’’" := ttVar0 : well_typed_term_scope.
+
+  Axiom tVar0 : Preterm.
+  Notation "‘VAR₀’" := tVar0.
+
+End PretermPrimitives.
+
+Module Type PreL (LC : LobExtendedContext) (Export PP : PretermPrimitives LC).
+
+  Axiom App : forall {A' B' : Preterm},
+                □ (A' ‘→’ B') -> □ A' -> □ B'.
+
+  Axiom wttLambda_nd : forall {Γ : Context} {B' : Preterm},
+                       forall A' : Preterm, box' (Γ ▻ A') B' -> box' Γ (A' ‘→’ B').
+
+  Axiom wttApp_1_nd : forall {Γ : Context} {A' B' : Preterm},
+                        box' Γ (A' ‘→’ B') -> box' Γ A' -> box' Γ B'.
+
+  Notation "x ‘’ y" := (wttApp_1_nd x%wtt y%wtt) : well_typed_term_scope.
+
+  Axiom box'_weaken : forall {Γ A}, box' ε A -> box' Γ A.
+End PreL.
+
+Module Lob1 (LC : LobExtendedContext) (Import LH : LobHypotheses LC).
+
+  Module Type PretermPrimitives' := PretermPrimitives LC.
+
+  Module Type L (PP : PretermPrimitives') (Export PL : PreL LC PP).
+    Axiom L : Preterm.
+    Axiom qL : Preterm.
+    Notation "‘L’" := qL.
+  End L.
+
+  Module Type PostL (PP : PretermPrimitives') (PL : PreL LC PP) (Export L' : L PP PL).
+    Axiom Conv : □ (‘□’ ‘’ ⌜ L ⌝) -> □ (‘□’ ‘’ ‘L’).
+
+    Axiom Conv2 : □ L -> □ (‘□’ ‘’ ‘L’ ‘→’ ‘X’).
+    Axiom Conv2_inv : □ (‘□’ ‘’ ‘L’ ‘→’ ‘X’) -> □ L.
+    Axiom qConv2 : forall {Γ},
+                     box' Γ (‘□’ ‘’ ‘L’) -> box' Γ (‘□’ ‘’ (⌜ (‘□’ ‘’ ‘L’) ⌝ ‘‘→’’ ⌜ ‘X’ ⌝)).
+
+    Axiom Quot : □ L -> □ (‘□’ ‘’ ⌜ L ⌝).
+
+    Axiom qbApp
+    : forall (A' := (⌜ ‘□’ ‘’ ‘L’ ⌝)%preterm)
+             (B' := (⌜ ‘X’ ⌝)%preterm),
+        □ ((‘□’ ‘’ (A' ‘‘→’’ B')) ‘→’ ‘□’ ‘’ A' ‘→’ ‘□’ ‘’ B').
+
+    Notation "‘‘App’’" := (box'_weaken qbApp) : well_typed_term_scope.
+
+    (*Axiom qConv
+  : □ (‘□’ ‘’ ⌜‘□’ ‘’ ⌜L ⌝ ⌝ ‘→’ ‘□’ ‘’ ⌜ ‘□’ ‘’ ‘L’ ⌝).
+
+  Notation "‘‘Conv’’" := (box'_weaken qConv) : well_typed_term_scope.*)
+
+    Axiom qQuote
+    : let A := (‘□’ ‘’ ‘L’)%preterm in
+      □ (A ‘→’ (‘□’ ‘’ (⌜ A ⌝))).
+
+    Notation "‘‘Quote’’" := (box'_weaken qQuote) : well_typed_term_scope.
+  End PostL.
+End Lob1.
+
+Module Type Lob1H (Export LC : LobExtendedContext) (Export LH : LobHypotheses LC).
+  Module Lob1' := Lob1 LC LH.
+  Declare Module Export PP : PretermPrimitives LC.
+  Declare Module Export PreL' : PreL LC PP.
+  Declare Module Export L' : Lob1'.L PP PreL'.
+  Declare Module Export PostL' : Lob1'.PostL PP PreL' L'.
+End Lob1H.
+
+Module Lob1' (LC : LobExtendedContext) (Import LH : LobHypotheses LC) (Import M : Lob1H LC LH)
+<: LobsTheorem LC LH.
+  Notation "‘‘f’’" := (box'_weaken wtt_qf) : well_typed_term_scope.
+
+  Definition lob : X.
+    refine ((fun (ℓ : □ L) => f (App (Conv2 ℓ) (Conv (Quot ℓ))))
+              (Conv2_inv
+                 (wttLambda_nd
+                    (‘□’ ‘’ ‘L’)
+                    (‘‘f’’ ‘’ ((‘‘App’’ ‘’ (qConv2 ‘‘VAR₀’’)) ‘’ ((*‘‘Conv’’ ‘’*) (‘‘Quote’’ ‘’ ‘‘VAR₀’’))))))).
+  Defined.
+End Lob1'.
+
+Module Type PretermReflectionPrimitives (Export LC : LobExtendedContext).
+  Axiom qPreterm : Preterm.
+  Notation "‘Preterm’" := qPreterm : preterm_scope.
+
+  Axiom qquote : Preterm.
+  Notation "‘quote’" := qquote : preterm_scope.
+End PretermReflectionPrimitives.
+
+Module Type TypingRules (Export LC : LobExtendedContext) (Export PP : PretermPrimitives LC).
+  Axiom capture_avoiding_subst_0 : forall (in_term : Preterm)
+                                          (new_value : Preterm),
+                                     Preterm.
+  Notation "x [ 0 ↦ y ]" := (capture_avoiding_subst_0 x y).
+  Axiom convertible : Context -> Preterm -> Preterm -> Prop.
+  Axiom box'_respectful : forall {Γ A B},
+                            convertible Γ A B
+                            -> box' Γ A
+                            -> box' Γ B.
+  Axiom convertible_refl : forall {Γ}, Reflexive (convertible Γ).
+  Axiom convertible_sym : forall {Γ}, Symmetric (convertible Γ).
+  Axiom convertible_trans : forall {Γ}, Transitive (convertible Γ).
+  Axiom convertible_tApp : forall {Γ A A' B B'},
+                             convertible Γ A A'
+                             -> convertible Γ B B'
+                             -> convertible Γ (tApp A B) (tApp A' B').
+  Axiom convertible_beta_app_lambda
+  : forall Γ A f a,
+      convertible Γ (tApp (tLambda A f) a) (capture_avoiding_subst_0 f a).
+  Axiom convertible__capture_avoiding_subst_0__tApp
+  : forall Γ A B x,
+      convertible Γ ((A ‘’ B) [ 0 ↦ x ]) ((A [ 0 ↦ x ]) ‘’ (B [ 0 ↦ x ])).
+  Axiom convertible__capture_avoiding_subst_0__qtProd
+  : forall Γ A B x,
+      convertible Γ ((A ‘‘→’’ B) [ 0 ↦ x ]) ((A [ 0 ↦ x ]) ‘‘→’’ (B [ 0 ↦ x ])).
+  Axiom convertible__capture_avoiding_subst_0__tVar0
+  : forall Γ x,
+      convertible Γ (‘VAR₀’ [ 0 ↦ x ]) x.
+
+  Axiom qtProd_Proper_convertible
+  : forall Γ,
+      Proper (convertible Γ ==> convertible Γ ==> convertible Γ) qtProd.
+  Existing Instance qtProd_Proper_convertible.
+  Axiom tApp_Proper_convertible
+  : forall Γ,
+      Proper (convertible Γ ==> convertible Γ ==> convertible Γ) tApp.
+  Existing Instance tApp_Proper_convertible.
+  Axiom convertible__quote__qtProd
+  : forall Γ A B,
+      convertible Γ (⌜ A ‘→’ B ⌝) (⌜ A ⌝ ‘‘→’’ ⌜ B ⌝).
+  Axiom convertible__quote__closed
+  : forall Γ A x,
+      convertible Γ ((quote A) [ 0 ↦ x ]) (quote A).
+  Axiom convertible__qtApp__closed
+  : forall Γ x,
+      convertible Γ (‘App’ [ 0 ↦ x ]) (‘App’).
+  Axiom convertible__quote__app
+  : forall Γ A B,
+      convertible Γ (⌜ A ‘’ B ⌝) ((‘App’ ‘’ ⌜ A ⌝) ‘’ ⌜ B ⌝).
+End TypingRules.
+
+Module Type PretermReflectionTypingRules (Export LC : LobExtendedContext) (Export PP : PretermPrimitives LC) (Export PRP : PretermReflectionPrimitives LC) (Export TR : TypingRules LC PP).
+  Axiom convertible__qquote__closed
+  : forall Γ x,
+      convertible Γ (‘quote’ [ 0 ↦ x ]) (‘quote’).
+
+  (*Axiom box_distr_qtProd_quote
+  : forall Γ A B,
+      convertible Γ (‘□’ ‘’ (A ‘‘→’’ ⌜ B ⌝)) ((‘□’ ‘’ A) ‘‘→’’ (‘□’ ‘’ ⌜ B ⌝)).*)
+
+  Axiom box_qtProd_dom_precompose
+  : forall {Γ} A B C,
+      (box' Γ (‘□’ ‘’ B) -> box' Γ (‘□’ ‘’ A))
+      -> box' Γ (‘□’ ‘’ (A ‘‘→’’ C))
+      -> box' Γ (‘□’ ‘’ (B ‘‘→’’ C)).
+
+  (** FIXME: This seems a bit fishy... *)
+  Axiom box_quote_app_quote
+  : forall Γ T,
+      box' Γ (‘□’
+               ‘’ (‘App’ ‘’ ⌜‘□’ ⌝ ‘’ (‘App’ ‘’ ⌜T ⌝ ‘’ (‘App’ ‘’ ‘quote’ ‘’ ⌜ T ⌝))))
+      -> box' Γ (‘□’ ‘’ (‘App’ ‘’ ⌜‘□’ ⌝ ‘’ (‘App’ ‘’ ⌜T ⌝ ‘’ ⌜ ⌜ T ⌝ ⌝))).
+
+  Axiom box_quote_app_quote_inv
+  : forall Γ T,
+      box' Γ (‘□’ ‘’ (‘App’ ‘’ ⌜‘□’ ⌝ ‘’ (‘App’ ‘’ ⌜T ⌝ ‘’ ⌜ ⌜ T ⌝ ⌝)))
+      -> box' Γ (‘□’
+                  ‘’ (‘App’ ‘’ ⌜‘□’ ⌝ ‘’ (‘App’ ‘’ ⌜T ⌝ ‘’ (‘App’ ‘’ ‘quote’ ‘’ ⌜ T ⌝)))).
+End PretermReflectionTypingRules.
+
+Module Type PostL_Assumptions (LC : LobExtendedContext) (Export PP : PretermPrimitives LC).
+  Axiom Quot : forall T, □ T -> □ (‘□’ ‘’ ⌜ T ⌝).
+
+  Axiom qQuote
+  : forall T,
+      let A := (‘□’ ‘’ T)%preterm in
+      □ (A ‘→’ (‘□’ ‘’ (⌜ A ⌝))).
+
+  Axiom qbApp
+   : forall A' B',
+       □ ((‘□’ ‘’ (A' ‘‘→’’ B')) ‘→’ (‘□’ ‘’ A') ‘→’ (‘□’ ‘’ B')).
+End PostL_Assumptions.
+
+Module Lob2 (LC : LobExtendedContext) (Import LH : LobHypotheses LC).
+  Module Lob1' := Lob1 LC LH.
+
+  Module L (Export PP : PretermPrimitives LC) (Export PL : PreL LC PP) (Export PRP : PretermReflectionPrimitives LC) (Export TR : TypingRules LC PP) (Export PRTR : PretermReflectionTypingRules LC PP PRP TR)
+  <: Lob1'.L PP PL.
+
+    Definition L0 (h : Preterm) : Preterm
+      := ((‘□’ ‘’ (h ‘’ (quote h))) ‘→’ ‘X’)%preterm.
+
+    Definition qL0 : Preterm
+      := tLambda
+           ‘Preterm’
+           (((‘App’ ‘’ ⌜ ‘□’ ⌝)
+               ‘’ ((‘App’ ‘’ ‘VAR₀’ ‘’ (‘App’ ‘’ ‘quote’ ‘’ ‘VAR₀’))))
+              ‘‘→’’
+              ⌜ ‘X’ ⌝).
+
+    Notation "‘L0’" := qL0.
+
+    Definition L : Preterm
+      := L0 ‘L0’.
+
+    Definition qL : Preterm
+      := ‘L0’ ‘’ ⌜ ‘L0’ ⌝.
+
+    Notation "‘L’" := qL.
+  End L.
+
+  Module PostL (Export PP : PretermPrimitives LC) (Export PL : PreL LC PP) (Export PRP : PretermReflectionPrimitives LC) (Export TR : TypingRules LC PP) (Export PRTR : PretermReflectionTypingRules LC PP PRP TR) (LA : PostL_Assumptions LC PP).
+    Module L' := L PP PL PRP TR PRTR.
+    Include L'.
+
+    Module M <: Lob1'.PostL PP PL L'.
+
+      Local Ltac conv_rewrite
+        := repeat match goal with
+                    | [ |- convertible _ ?x ?x ] => reflexivity
+                    | [ |- convertible _ (?x ‘’ _) (?x ‘’ _) ]
+                      => apply tApp_Proper_convertible; [ reflexivity | ]
+                    | [ |- convertible _ (_ ‘‘→’’ _) (_ ‘‘→’’ _) ]
+                      => apply qtProd_Proper_convertible
+                    | _ => progress rewrite ?convertible__capture_avoiding_subst_0__tApp, ?convertible__qtApp__closed, ?convertible__quote__closed, ?convertible__quote__app, ?convertible__capture_avoiding_subst_0__tVar0, ?convertible__qquote__closed, ?convertible__capture_avoiding_subst_0__qtProd, ?convertible__quote__qtProd, ?convertible_beta_app_lambda
+                  end.
+
+      Definition Conv : □ (‘□’ ‘’ ⌜ L ⌝) -> □ (‘□’ ‘’ ‘L’).
+      Proof.
+        unfold box, L, qL.
+        refine (fun box_L => let box_L' := box'_respectful _ box_L in _ box_L').
+        { unfold L0, qL0; conv_rewrite.
+          reflexivity. }
+        { clear.
+          unfold L0, qL0.
+          intro box_L.
+          eapply box'_respectful.
+          { conv_rewrite.
+            reflexivity. }
+          { revert box_L.
+            match goal with
+              | [ |- context[quote (quote ?X)] ] => generalize X; intro T
+            end.
+            apply box_qtProd_dom_precompose.
+            apply box_quote_app_quote. } }
+      Defined.
+
+      Definition Conv2 : □ L -> □ (‘□’ ‘’ ‘L’ ‘→’ ‘X’)
+        := fun x => x.
+      Definition Conv2_inv : □ (‘□’ ‘’ ‘L’ ‘→’ ‘X’) -> □ L
+        := fun x => x.
+      Definition qConv2 {Γ}
+      : box' Γ (‘□’ ‘’ ‘L’) -> box' Γ (‘□’ ‘’ (⌜‘□’ ‘’ ‘L’ ⌝ ‘‘→’’ ⌜ ‘X’ ⌝)).
+      Proof.
+        unfold qL.
+        refine (fun box_L => let box_L' := box'_respectful _ box_L in _ box_L').
+        { unfold L0, qL0; conv_rewrite.
+          reflexivity. }
+        { clear.
+          unfold L0, qL0.
+          intro box_L.
+          eapply box'_respectful.
+          { conv_rewrite.
+            reflexivity. }
+          { revert box_L.
+            match goal with
+              | [ |- context[quote (quote ?X)] ] => generalize X; intro T
+            end.
+            apply box_qtProd_dom_precompose.
+            apply box_quote_app_quote_inv. } }
+      Defined.
+
+      (*Axiom qConv
+  : □ (‘□’ ‘’ ⌜‘□’ ‘’ ⌜L ⌝ ⌝ ‘→’ ‘□’ ‘’ ⌜ ‘□’ ‘’ ‘L’ ⌝).
+
+  Notation "‘‘Conv’’" := (box'_weaken qConv) : well_typed_term_scope.*)
+
+      Definition Quot : □ L -> □ (‘□’ ‘’ ⌜ L ⌝)
+        := LA.Quot _.
+
+      Definition qbApp
+      : forall (A' := (⌜‘□’ ‘’ ‘L’ ⌝)%preterm)
+               (B' := (⌜‘X’ ⌝)%preterm),
+          □ ((‘□’ ‘’ (A' ‘‘→’’ B')) ‘→’ (‘□’ ‘’ A') ‘→’ (‘□’ ‘’ B'))
+        := LA.qbApp _ _.
+
+      Notation "‘‘App’’" := (box'_weaken qbApp) : well_typed_term_scope.
+
+      Definition qQuote
+      : let A := (‘□’ ‘’ ‘L’)%preterm in
+        □ (A ‘→’ (‘□’ ‘’ (⌜ A ⌝)))
+        := LA.qQuote _.
+
+      Notation "‘‘Quote’’" := (box'_weaken qQuote) : well_typed_term_scope.
+    End M.
+  End PostL.
+End Lob2.
+
+Module Type Lob2H (Export LC : LobExtendedContext) (Export LH : LobHypotheses LC).
+  Module Lob2' := Lob2 LC LH.
+  Declare Module Export PP : PretermPrimitives LC.
+  Declare Module Export PreL' : PreL LC PP.
+  Declare Module Export PRP : PretermReflectionPrimitives LC.
+  Declare Module Export TR : TypingRules LC PP.
+  Declare Module Export PRTR : PretermReflectionTypingRules LC PP PRP TR.
+  Declare Module Export LA : PostL_Assumptions LC PP.
+End Lob2H.
+
+Module Lob2'0 (LC : LobExtendedContext) (LH : LobHypotheses LC) (M : Lob2H LC LH)
+<: LobsTheorem LC LH.
+  Module Lob1HV <: Lob1H LC LH.
+    Include M.
+    Include M.Lob2'.
+    Module L' <: Lob1'.L PP PreL'
+      := L PP PreL' PRP TR PRTR.
+    Module PostL'' := M.Lob2'.PostL PP PreL' PRP TR PRTR LA.
+    Module PostL' <: Lob1'.PostL PP PreL' L'
+      := PostL''.M.
+  End Lob1HV.
+  Module M' := Lob1' LC LH Lob1HV.
+  Definition lob := M'.lob.
+End Lob2'0.
+
+Module LobOfPreLob
+       (Export LC : LobExtendedContext)
+       (Export LH : LobHypotheses LC)
+       (Export PP : PretermPrimitives LC)
+       (Export PreL' : PreL LC PP)
+       (Export PRP : PretermReflectionPrimitives LC)
+       (Export TR : TypingRules LC PP)
+       (Export PRTR : PretermReflectionTypingRules LC PP PRP TR)
+       (Export LA : PostL_Assumptions LC PP)
+<: LobsTheorem LC LH.
+  Module M'0 <: Lob2H LC LH.
+    Module Lob2' := Lob2 LC LH.
+    Module PP := PP.
+    Module PreL' := PreL'.
+    Module PRP := PRP.
+    Module TR := TR.
+    Module PRTR := PRTR.
+    Module LA := LA.
+  End M'0.
+  Include (Lob2'0 LC LH M'0).
+End LobOfPreLob.
